templates/hindsight_module/hindsight_proof.v
@@ -8,229 +8,14 @@ From iris.heap_lang Require Import proofmode par.
 From iris.heap_lang.lib Require Import nondet_bool.
 From iris.bi.lib Require Import fractional.
 From diaframe.heap_lang Require Import proof_automation atomic_specs wp_auto_lob.
-Require Export one_shot_proph typed_proph.
+Require Export hindsight.
 
-Module Type DATA_STRUCTURE.
-  
-  Parameter dsOp : val.
-  Parameter Op : Type.
-  Parameter Op_to_val : Op -> val.
+Module Type HINDSIGHT_SPEC (ADT: ABSTRACT_DATA_TYPE) (DS : DATA_STRUCTURE ADT).
+  Module DEFS := HINDSIGHT_DEFS ADT DS.
+  Import ADT DS DEFS.
 
-  Parameter snapshotUR : ucmra.
-  Definition snapshot := ucmra_car snapshotUR.
-
-  Parameter absTUR : ucmra.
-  Definition absT := ucmra_car absTUR.
-
-  Parameter resT : Type.
-  Parameter resT_to_base_lit : resT -> base_lit.
-  Coercion resT_to_base_lit : resT >-> base_lit.
-  Parameter resT_from_val : val -> option resT.
-  Parameter resT_to_val : resT -> val.
-  Parameter resT_inj_prop : ∀ (r : resT), resT_from_val (resT_to_val r) = Some r.
-  Definition resTProph : TypedProphSpec :=
-    mkTypedProphSpec resT resT_from_val resT_to_val resT_inj_prop.
-  Definition resTTypedProph `{!heapGS Σ} := make_TypedProph resTProph.
-  Parameter resT_proph_resolve : ∀ (res: resT), resT_from_val #res = Some res.
-  
-  Parameter seq_spec : Op -> absT -> absT -> resT -> Prop.
-  Parameter abs : snapshot -> absT.
-  Parameter updater_thread: Op -> resT -> bool.
-
-  Parameter neg_seq_spec_dec : ∀ op c c' res, Decision (¬ seq_spec op c c' res).
-  Parameter seq_spec_dec : ∀ op c c' res, Decision (seq_spec op c c' res).
-  Parameter updater_thread_dec: ∀ op res b, Decision (updater_thread op res = b).  
-  
-  Parameter snapshotUR_discrete : CmraDiscrete snapshotUR.
-  Parameter absTUR_discrete : CmraDiscrete absTUR.
-  Parameter snapshot_leibnizequiv : LeibnizEquiv (snapshot).
-  Parameter snapshot_inhabited : Inhabited snapshot.
-  Parameter resT_inhabited : Inhabited resT.
-  Parameter Op_inhabited : Inhabited Op.
-  
-End DATA_STRUCTURE.  
-
-Module HINDSIGHT_DEFS (DS : DATA_STRUCTURE).
-  Import DS.
-  
-  Global Instance snapshotUR_discrete' : CmraDiscrete snapshotUR.
-  Proof.
-    apply snapshotUR_discrete.
-  Qed.
-  
-  Global Instance absTUR_discrete' : CmraDiscrete absTUR.
-  Proof.
-    apply absTUR_discrete.
-  Qed.
-
-  Global Instance snapshot_leibnizequiv' : LeibnizEquiv (snapshot).
-  Proof.
-    apply snapshot_leibnizequiv.
-  Qed.  
-
-  Global Instance snapshot_inhabited' : Inhabited snapshot.
-  Proof.
-    apply snapshot_inhabited.
-  Qed.
-
-  Global Instance resT_inhabited' : Inhabited resT.
-  Proof.
-    apply resT_inhabited.
-  Qed.
-
-  Global Instance Op_inhabited' : Inhabited Op.
-  Proof.
-    apply Op_inhabited.
-  Qed.
-
-  
-  (* RAs used in proof *)
-
-  Definition auth_natUR := authUR $ max_natUR.
-  Definition agree_snapshotR := agreeR $ snapshotUR.
-  Definition frac_absTR := dfrac_agreeR $ absTUR.
-  Definition historyR := gmapUR nat $ snapshotUR.
-  Definition auth_historyR := authR $ gmapUR nat $ agree_snapshotR.
-  Definition frac_historyR := dfrac_agreeR $ historyR.
-  Definition tokenUR := exclR unitO.
-  Definition set_tidR := authR (gsetUR proph_id). 
-  Definition thread_viewR := authUR $ 
-                              gmapUR proph_id $ 
-                                agreeR $ prodO natO gnameO.
-
-  Class dsG Σ := DS {
-                  dsG_auth_natG :> inG Σ auth_natUR;
-                  dsG_agree_snapshotG :> inG Σ agree_snapshotR;
-                  dsG_frac_absTG :> inG Σ frac_absTR;
-                  dsG_historyG :> inG Σ historyR;
-                  dsG_auth_historyG :> inG Σ auth_historyR;
-                  dsG_tokenG :> inG Σ tokenUR;
-                  dsG_frac_historyG :> inG Σ frac_historyR;
-                  dsG_set_tidG :> inG Σ set_tidR;
-                  dsG_thread_viewG :> inG Σ thread_viewR
-                 }.
-                 
-  Definition dsΣ : gFunctors :=
-    #[ GFunctor auth_natUR; GFunctor agree_snapshotR;
-       GFunctor frac_absTR; GFunctor historyR;
-       GFunctor auth_historyR; GFunctor tokenUR; 
-       GFunctor frac_historyR; GFunctor set_tidR;
-       GFunctor thread_viewR ].
-  
-  Global Instance subG_dsΣ {Σ} : subG dsΣ Σ → dsG Σ.
-  Proof. solve_inG. Qed.
-
-  Context {Σ} `{!heapGS Σ, !dsG Σ}.
-  Notation iProp := (iProp Σ).
-  Implicit Types M : gmap nat snapshot.
-  Implicit Types T : nat.
-  
-  Global Definition cntrN N := N .@ "cntr".
-  Global Definition threadN N := N .@ "thread".
-  
-
-  Definition map_max (M: gmap nat snapshot) : nat := 
-    max_list (elements (dom M)).
-
-  Definition hist γ_t γ_m M T : iProp :=
-    ∃ (M': gmap nat (agreeR (_))),
-      own γ_t (● MaxNat T) ∗ own γ_m (● M')
-    ∗ ⌜T = map_max M⌝
-    ∗ ⌜map_Forall (λ k a, a = to_agree (M !!! k)) M'⌝
-    ∗ ⌜∀ t, t < T → M !!! t ≠ M !!! (t+1)%nat⌝.
-
-  Definition dsRep γ_s (a: absTUR) : iProp := 
-    own γ_s (to_frac_agree (1/2) a).
-
-  Definition dsRepI γ_s (a: absTUR) : iProp := 
-    own γ_s (to_frac_agree (1/2) a).
-    
-  (** Helping Inv **)
-  
-  Definition au N γ_r op (Q : val → iProp) := 
-    (AU << ∃∃ a, dsRep γ_r a >> 
-          @ ⊤ ∖ ↑(cntrN N), ∅
-        << ∀∀ a' res, dsRep γ_r a' ∗ ⌜seq_spec op a a' res⌝, COMM Q #res >>)%I.
-        
-  Definition past_lin M T op res t0 : iProp :=
-    ⌜match updater_thread op res with
-    | true =>
-      ∃ t, t0 ≤ t < T ∧ seq_spec op (abs (M !!! t)) (abs (M !!! (t+1)%nat)) res
-    | false =>  
-      ∃ t, t0 ≤ t ≤ T ∧ seq_spec op (abs (M !!! t)) (abs (M !!! t)) res end⌝.
-
-  Definition past_state γ_m (t0: nat) (s: snapshot) : iProp :=
-    ∃ t, ⌜t0 ≤ t⌝ ∗ own γ_m (◯ {[t := to_agree s]}).
-  
-  Definition past_two_states γ_m (t0: nat) (s s': snapshot) : iProp :=
-    ∃ t, ⌜t0 ≤ t⌝ 
-    ∗ own γ_m (◯ {[t := to_agree s]}) 
-    ∗ own γ_m (◯ {[t+1 := to_agree s']}).
-
-  Definition past_lin_witness γ_m op res t0 : iProp :=
-    match updater_thread op res with
-    | true =>
-      ∃ s s', past_two_states γ_m t0 s s' ∗ ⌜seq_spec op (abs s) (abs s') res⌝
-    | false =>  
-      ∃ s, past_state γ_m t0 s ∗ ⌜seq_spec op (abs s) (abs s) res⌝ end.
-
-  Definition Pending (P: iProp) M T op vp t0 : iProp := 
-    P ∗ £1 ∗ ¬ past_lin M T op vp t0.
-
-  Definition Done γ_tk (Q: val → iProp) M T op (vp: resT) t0 : iProp := 
-      (Q #vp ∨ own γ_tk (Excl ())) ∗ past_lin M T op vp t0.
-
-  Definition State γ_sy γ_tk P Q M T op vp t0 : iProp :=
-      own γ_sy (to_frac_agree (1/2) M)
-    ∗ ⌜T = map_max M⌝ 
-    ∗ (Pending P M T op vp t0 ∨ Done γ_tk Q M T op vp t0).
-
-  Definition thread_vars γ_t γ_ght γ_sy t_id t0 : iProp := 
-    own γ_ght (◯ {[t_id := to_agree (t0, γ_sy)]}) ∗ own γ_t (◯ MaxNat t0).
-
-  Definition Reg N γ_t γ_s γ_ght t_id M : iProp :=
-    ∃ γ_tk γ_sy Q op vp t0 (vtid: val), 
-        proph1 t_id vtid
-      ∗ thread_vars γ_t γ_ght γ_sy t_id t0
-      ∗ own (γ_sy) (to_frac_agree (1/2) M)
-      ∗ inv (threadN N) (∃ M T, State γ_sy γ_tk (au N γ_s op Q) Q M T op vp t0).
-
-  Definition helping_inv (N: namespace) γ_t γ_s γ_td γ_ght M : iProp :=
-    ∃ (R: gset proph_id) (hγt: gmap proph_id (agreeR _)),
-        own γ_td (● R)
-      ∗ own γ_ght (● hγt) ∗ ⌜dom hγt = R⌝  
-      ∗ ([∗ set] t_id ∈ R, Reg N γ_t γ_s γ_ght t_id M).
-  
-  Definition ds_inv N γ_t γ_s γ_m γ_td γ_ght template_inv : iProp :=
-    inv (cntrN N)
-    (∃ M T (s: snapshot),
-      dsRepI γ_s (abs s) ∗ ⌜abs (M !!! T) = abs s⌝
-    ∗ hist γ_t γ_m M T
-    ∗ helping_inv N γ_t γ_s γ_td γ_ght M
-    ∗ template_inv M T s).
-(*    
-  Instance dsRep_timeless : ∀ γ_s C, Timeless (dsRep γ_s C).
-  Proof.
-    intros γ_s C. rewrite /dsRep. Search Timeless. 
-    apply own_timeless; apply _.
-  Qed.   
-*)    
-  Definition update_helping_protocol N γ_t γ_s γ_td γ_ght : iProp :=
-        ∀ M T n s, 
-          ⌜map_max M = T⌝ -∗   
-            dsRep γ_s n -∗ own γ_t (● MaxNat T) -∗ 
-              helping_inv N γ_t γ_s γ_td γ_ght M ={⊤ ∖ ↑cntrN N}=∗
-                helping_inv N γ_t γ_s γ_td γ_ght (<[T := s]> M) 
-                ∗ dsRep γ_s n ∗ own γ_t (● MaxNat T).
-    
-End HINDSIGHT_DEFS.
-
-Module Type HINDSIGHT_SPEC (DS : DATA_STRUCTURE).
-  Module DEFS := HINDSIGHT_DEFS DS.
-  Import DEFS DS.
-
-  Parameter dsOp_spec: ∀ N γ_s γ_t γ_m γ_td γ_ght template_inv op r γ_sy t_id t0,
-          ds_inv N γ_t γ_s γ_m γ_td γ_ght template_inv -∗
+  Parameter dsOp_spec: ∀ N γ_s γ_t γ_m γ_td γ_ght op (r: Node) γ_sy t_id t0,
+          main_inv N γ_t γ_s γ_m γ_td γ_ght -∗
             □ update_helping_protocol N γ_t γ_s γ_td γ_ght -∗
               thread_vars γ_t γ_ght γ_sy t_id t0 -∗
                 {{{ True }}} 
@@ -239,9 +24,10 @@ Module Type HINDSIGHT_SPEC (DS : DATA_STRUCTURE).
 
 End HINDSIGHT_SPEC.
 
-Module CLIENT_SPEC (DS : DATA_STRUCTURE) (HS: HINDSIGHT_SPEC DS).
-(*   Module DEFS := HINDSIGHT_DEFS DS. *)
-  Import HS DEFS DS.
+Module CLIENT_SPEC (ADT: ABSTRACT_DATA_TYPE) (DS : DATA_STRUCTURE ADT) 
+  (HS: HINDSIGHT_SPEC ADT DS).
+  (* Module DEFS := HINDSIGHT_DEFS ADT DS. *)
+  Import ADT DS HS DEFS.
 
   Definition dsOp' : val :=
     λ: "OP" "r",     
@@ -253,8 +39,8 @@ Module CLIENT_SPEC (DS : DATA_STRUCTURE) (HS: HINDSIGHT_SPEC DS).
         
   (** Proofs *)
 
-  Lemma dsOp'_spec N γ_s γ_t γ_m γ_td γ_ght template_inv op r :
-          ds_inv N γ_t γ_s γ_m γ_td γ_ght template_inv -∗
+  Lemma dsOp'_spec N γ_s γ_t γ_m γ_td γ_ght op (r: Node) :
+          main_inv N γ_t γ_s γ_m γ_td γ_ght -∗
               <<< ∀∀ a, dsRep γ_s a >>> 
                      dsOp' (Op_to_val op) #r @ ↑(cntrN N)
               <<< ∃∃ a' res, dsRep γ_s a' ∗ ⌜seq_spec op a a' res⌝, RET #res >>>.
@@ -316,6 +102,8 @@ Module CLIENT_SPEC (DS : DATA_STRUCTURE) (HS: HINDSIGHT_SPEC DS).
     iAssert (own γ_t (◯ (MaxNat T0))) as "HfragT0".
     { admit. }
     
+    assert (∀ op c c' res, Decision (¬ seq_spec op c c' res)) as neg_seq_spec_dec.
+    { intros; apply not_dec. apply seq_spec_dec. }
     assert (∀ op c res, Decision (updater_thread op res = true 
               ∨ (updater_thread op res = false 
                   ∧ ¬ seq_spec op c c res))) as Hdec.
@@ -361,7 +149,7 @@ Module CLIENT_SPEC (DS : DATA_STRUCTURE) (HS: HINDSIGHT_SPEC DS).
       { admit. }
       iAssert (thread_vars γ_t γ_ght γ_sy tid T0)%I as "#Thr_vars".
       { iFrame "#". }
-
+      Check dsOp_spec.
       wp_apply dsOp_spec; try done.
       iIntros (res)"HpastW".
       wp_pures.
@@ -510,20 +298,6 @@ Module CLIENT_SPEC (DS : DATA_STRUCTURE) (HS: HINDSIGHT_SPEC DS).
       { unfold typed_proph_from_val; simpl. by rewrite resT_proph_resolve. }    
       wp_pures. iModIntro. iIntros "->".
       wp_pures. iModIntro. done. 
-    
   Admitted.
   
-End CLIENT_SPEC.  
-  
-  
-  
-  
-  
-  
-  
-  
-  
-  
-  
-  
-  
+End CLIENT_SPEC.
