templates/hindsight_module/search_structures.v
@@ -1,0 +1,102 @@
+(*
+Differences compared to hindsight.v:
+
+1) History needs to be updated anytime a snapshot is 
+  updated (and not just when the abstract state is udpated).
+2) M !!! T = s -> M !!! T ≡ s
+*)
+
+From iris.algebra Require Import excl auth cmra gmap agree gset numbers.
+From iris.algebra.lib Require Import dfrac_agree.
+From iris.heap_lang Require Export notation locations lang.
+From iris.base_logic.lib Require Export invariants fancy_updates.
+From iris.program_logic Require Export atomic.
+From iris.proofmode Require Import tactics.
+From iris.heap_lang Require Import proofmode par.
+From iris.heap_lang.lib Require Import nondet_bool.
+From iris.bi.lib Require Import fractional.
+From diaframe.heap_lang Require Import proof_automation atomic_specs wp_auto_lob.
+Require Export hindsight.
+
+Module SEARCH_STRUCTURE : ABSTRACT_DATA_TYPE with Definition absTUR := gsetUR nat.
+
+  Parameter search : val.
+  Parameter insert : val.
+  Parameter delete : val.
+
+  Definition dsOp : val :=
+    λ: "OP" "r" "k",     
+      if: "OP" = #0 
+      then search "r" "k"
+      else if: "OP" = #1 
+      then insert "r" "k"
+      else delete "r" "k".
+
+  (* Definition K := Z. *)
+  Inductive Opp := searchOp : nat → Opp | insertOp : nat → Opp | deleteOp : nat → Opp.
+  Definition Op := Opp.
+
+  Definition Op_to_val (op: Op) : val :=
+    match op with
+    | searchOp _ => #0
+    | insertOp _ => #1
+    | deleteOp _ => #2 
+    end.
+    
+  Definition absTUR := gsetUR nat.
+  Definition absT := ucmra_car absTUR.
+
+  Definition resT := bool.
+  Definition resT_to_base_lit (b: resT) : base_lit := LitBool b.
+  Coercion resT_to_base_lit : resT >-> base_lit.
+  Definition resT_from_val (v : val) : option bool :=
+    match v with
+    | LitV(LitBool b) => Some b
+    | _               => None
+    end.
+  Definition resT_to_val (b : bool) : val := LitV(LitBool b).
+  
+  Lemma resT_inj_prop : ∀ (b : bool), bool_from_val (bool_to_val b) = Some b.
+  Proof. done. Qed.
+
+  Definition resTProph : TypedProphSpec :=
+    mkTypedProphSpec resT resT_from_val resT_to_val resT_inj_prop.
+  Definition resTTypedProph `{!heapGS Σ} := make_TypedProph resTProph.
+
+  Lemma resT_proph_resolve : ∀ (res: resT), resT_from_val #res = Some res.
+  Proof. try done. Qed.
+
+  Definition seq_spec (op: Op) (C: absT) (C': absT) (res: bool) : Prop :=
+    match op with
+    | searchOp k => C' = C ∧ (if res then k ∈ C else k ∉ C)
+    | insertOp k => C' = C ∪ {[k]} ∧ (if res then k ∉ C else k ∈ C)
+    | deleteOp k => C' = C ∖ {[k]} ∧ (if res then k ∈ C else k ∉ C)
+    end.
+
+  Global Instance seq_spec_dec : ∀ op c c' res, Decision (seq_spec op c c' res).
+  Proof.
+    intros op c c' res. unfold seq_spec. 
+    destruct op; try apply and_dec; try destruct res; try apply _.
+  Qed.
+
+  Definition updater_thread (op: Op) (res: resT) : bool := 
+    match op, res with
+    | searchOp _, _ => false
+    | _, false => false
+    | _, _ => true
+    end.
+
+  Global Instance updater_thread_dec: ∀ op res b, 
+    Decision (updater_thread op res = b).
+  Proof.
+    intros op res b. unfold updater_thread.
+    destruct op; destruct res; try apply _.
+  Qed.  
+
+  Global Instance Op_inhabited : Inhabited Op := populate (searchOp 0).
+  Global Instance absTUR_discrete : CmraDiscrete absTUR.
+  Proof. try apply _. Qed.
+  Global Instance resT_inhabited : Inhabited resT.
+  Proof. try apply _. Qed.
+
+End SEARCH_STRUCTURE.
