templates/hindsight_module/skiplist_v0.v
@@ -1,0 +1,269 @@
+(* Herlihy Skiplist with a single level *)
+
+From iris.algebra Require Import excl auth cmra gmap agree gset numbers.
+From iris.algebra.lib Require Import dfrac_agree.
+From iris.heap_lang Require Export notation locations lang.
+From iris.base_logic.lib Require Export invariants.
+From iris.program_logic Require Export atomic.
+From iris.proofmode Require Import tactics.
+From iris.heap_lang Require Import proofmode par.
+From iris.heap_lang.lib Require Import nondet_bool.
+From iris.bi.lib Require Import fractional.
+Set Default Proof Using "All".
+From iris.bi.lib Require Import fractional.
+(* From diaframe.heap_lang Require Import proof_automation atomic_specs wp_auto_lob. *)
+Require Export search_structures hindsight_proof.
+
+Module SKIPLIST0 : DATA_STRUCTURE SEARCH_STRUCTURE.
+  Import SEARCH_STRUCTURE.
+  
+  (*
+    The snapshot stores:
+    0) set of nodes
+    1) ghost location for interface
+    2) global interface
+    3) ghost location for keyset
+    4) global contents
+    5) map from nodes to node-local info
+
+    Node local info:
+    1) singleton interface
+    2) keyset
+    3) physical contents
+    4) Marking
+  *)
+
+  
+  Definition snapshotUR := natUR.
+  Definition snapshot := ucmra_car snapshotUR.
+  
+  Definition abs (s: snapshot) : absT := ∅.
+
+  Global Instance snapshotUR_discrete : CmraDiscrete snapshotUR.
+  Proof. try apply _. Qed.
+
+  Global Instance snapshot_leibnizequiv : LeibnizEquiv (snapshot).
+  Proof. try apply _. Qed.
+  
+  Global Instance snapshot_inhabited : Inhabited snapshot := populate 0.
+  
+  Parameter inContents : val.
+  Parameter findNext : val.
+  Parameter try_constraint : val.
+  Parameter maintenance : val.
+  Parameter createNode: val.
+
+  (** Template algorithms *)
+
+  Definition traverse_rec (r: Node) : val :=
+    rec: "tr" "p" "c" "k" :=
+      let: "fn_ck" := findNext "c" "k" in
+      if: Fst "fn_ck" then
+        match: Snd "fn_ck" with
+          NONE => ""
+        | SOME "s" =>
+            match: try_constraint "p" "c" "s" with
+              NONE =>
+                let: "fn_hk" := findNext #r "k" in
+                match: Snd "fn_hk" with
+                  NONE => ""
+                | SOME "n" => 
+                    "tr" #r "n" "k" end
+            | SOME "_" => "tr" "p" "s" "k" end end  
+      else
+        match: Snd "fn_ck" with
+          NONE => ("p", "c")
+        | SOME "s" => "tr" "c" "s" "k" end.
+
+  Definition traverse (r: Node) : val := 
+    λ: "k", 
+      let: "fn_hk" := findNext #r "k" in
+      match: Snd "fn_hk" with
+        NONE => ""
+      | SOME "n" => 
+          traverse_rec r #r "n" "k" end.
+
+  Definition search (r: Node) : val :=
+    λ: "k",
+      let: "pc" := traverse r "k" in
+      let: "c" := Snd "pc" in
+      inContents "c" "k".
+      
+  Definition delete (r: Node) : val :=
+    λ: "k",
+      let: "pc" := traverse r "k" in
+      let: "c" := Snd "pc" in
+      if: ~ (inContents "c" "k") then
+        #false
+      else
+        match: try_constraint "c" with
+          NONE => #false
+        | SOME "_" => maintenance "k";; #true end.
+        
+  Definition insert (r: Node) : val :=
+    rec: "ins" "k" :=
+      let: "pc" := traverse r "k" in
+      let: "p" := Fst "pc" in
+      let: "c" := Snd "pc" in
+      if: inContents "c" "k" then
+        #false
+      else
+        let: "e" := createNode "k" "c" in
+        match: try_constraint "p" "c" "e" with
+          NONE => "ins" "k"
+        | SOME "_" => #true end.
+  
+  Definition esT : Type := gmap Node (gset nat).
+
+  Definition flowUR := authR (multiset_flowint_ur nat).
+  Definition auth_keysetUR := authUR $ (keysetUR nat).
+  Definition auth_setnodeUR := authUR $ (gsetUR Node).
+
+  Class dsGG Σ := ds {
+                    ds_flowG :> inG Σ flowUR;
+                    ds_auth_keysetG :> inG Σ auth_keysetUR;
+                    ds_auth_setnodeG :> inG Σ auth_setnodeUR;
+                   }.
+  
+  Definition dsG := dsGG.
+                
+                     
+  Definition dsΣ : gFunctors :=
+    #[ GFunctor flowUR;  GFunctor auth_keysetUR;
+       GFunctor auth_setnodeUR ].
+  
+  Global Instance subG_dsΣ {Σ} : subG dsΣ Σ → dsGG Σ.
+  Proof. solve_inG. Qed.
+
+    Context `{!heapGS Σ, !dsGG Σ}.
+    Context (γ_I γ_fp γ_ks: gname) (r: Node).
+    Notation iProp := (iProp Σ).
+  
+    Parameter node : Node → bool → esT → (gset nat) → iProp.
+    Parameter node_timeless_proof : ∀ r n es V, Timeless (node r n es V).
+    Global Instance node_timeless r n es V: Timeless (node r n es V).
+    Proof. apply node_timeless_proof. Qed.  
+
+    Parameter Mark : snapshot → Node → bool.
+    Parameter ES : snapshot → Node → esT.
+    Parameter PC : snapshot → Node → gset nat.
+    Parameter GFI : snapshot → (multiset_flowint_ur nat).
+    Parameter FI : snapshot → Node → (multiset_flowint_ur nat).
+    Parameter FP : snapshot → gset Node.
+  
+    Definition Cont (s: snapshot) (n: Node) : gset nat :=
+      if decide (Mark s n) then ∅ else PC s n.
+
+    Parameter out_set : multiset_flowint_ur nat → gset nat.
+    (* out_es es := ⋃_n es !!! n *)
+    Parameter out_es : esT → gset nat.
+    Parameter keyset : multiset_flowint_ur nat → gset nat. 
+    
+    (** data structure specific inv *)
+
+    Definition globalRes γ_I γ_fp γ_ks s : iProp :=
+        own γ_I (● (GFI s)) 
+      ∗ own γ_fp (● FP s) 
+      ∗ own γ_ks (● prod (KS, abs s)).
+    
+    Definition outflow_constraint (In: multiset_flowint_ur nat) (esn: esT) : Prop := True.
+  
+    Definition node_inv_pure s n : iProp :=
+        ⌜¬ (Mark s n) → out_set (FI s n) ⊆ inset nat (FI s n) n⌝
+      ∗ ⌜Cont s n ⊆ keyset (FI s n)⌝
+      ∗ ⌜Mark s n → out_set (FI s n) ≠ ∅⌝
+      ∗ ⌜outflow_constraint (FI s n) (ES s n)⌝ .
+
+    Definition node_inv γ_I γ_ks s n : iProp :=
+        node n (Mark s n) (ES s n) (PC s n)
+      ∗ own γ_I (◯ (FI s n))
+      ∗ own γ_ks (◯ prod (keyset (FI s n), Cont s n))
+      ∗ node_inv_pure s n.   
+
+    Definition per_tick_inv r s : iProp := 
+        ⌜inset nat (FI s r) r = KS⌝ ∗ ⌜out_set (FI s r) = KS⌝
+      ∗ ⌜¬ Mark s r⌝
+      ∗ [∗ set] n ∈ (FP s), node_inv_pure s n.
+    
+    Definition transition_inv s s' : Prop :=
+        (∀ n, n ∈ FP s → Mark s n → ES s' n = ES s n)
+      ∧ (∀ n, n ∈ FP s → Mark s n → Mark s' n)
+      ∧ (∀ n, n ∈ FP s → ¬ Mark s n → Mark s' n → ES s n ≠ ES s' n)
+      ∧ (∀ n, n ∈ FP s → PC s n = PC s' n)
+      ∧ (FP s ⊆ FP s').
+
+    
+
+    Definition ds_inv (M: gmap nat snapshot) 
+      (T: nat) (s: snapshot) : iProp :=
+        globalRes γ_I γ_fp γ_ks s
+      ∗ ([∗ set] n ∈ FP s, node_inv γ_I γ_ks s n)
+      ∗ ([∗ set] t ∈ dom M, per_tick_inv r (M !!! t))
+      ∗ ⌜∀ t, 0 ≤ t < T → transition_inv (M !!! t) (M !!! (t+1)%nat)⌝
+      ∗ ⌜transition_inv (M !!! T) s⌝.
+    
+    Global Instance ds_inv_timeless M T s : 
+      Timeless (ds_inv M T s).
+    Proof.
+    Admitted.  
+
+    (** Helper functions specs *)
+    
+    Parameter inContents_spec : ∀ (k: nat) (n: Node),
+       ⊢ (<<< ∀∀ m es pc, node n m es pc >>>
+             inContents #n #k @ ⊤
+         <<< ∃∃ (v: bool),
+                node n m es pc ∗ ⌜v ↔ k ∈ pc⌝,
+                RET #v >>>)%I.
+
+    Parameter findNext_spec : ∀ (k: nat) (n: Node),
+       ⊢ (<<< ∀∀ m es pc, node n m es pc >>>
+             findNext #n #k @ ⊤
+         <<< ∃∃ (success: bool) (n': Node),
+                node n m es pc
+              ∗ (match success with true => ⌜k ∈ es !!! n'⌝ 
+                                  | false => ⌜k ∉ out_es es⌝ end),
+             RET (match success with true => (#m, SOMEV #n') 
+                                   | false => (#m, NONEV) end)  >>>)%I.
+                                 
+    Definition edgset_update es k curr succ : esT :=
+      <[ succ := (es !!! succ) ∪ {[k]} ]>
+        (<[ curr := (es !!! curr) ∖ {[k]} ]> es).
+
+    Parameter try_constraint_trav_spec : ∀ (k: nat) (pred curr succ: Node),
+       ⊢ (<<< ∀∀ m es pc, node pred m es pc >>>
+             try_constraint #pred #curr #succ @ ⊤
+         <<< ∃∃ (success: bool) es',
+                node pred m es' pc
+              ∗ (match success with true => ⌜m = false⌝ ∗ ⌜k ∈ es !!! curr⌝
+                                            ∗ ⌜es' = edgset_update es k curr succ⌝ 
+                                  | false => ⌜m = true ∨ k ∉ es !!! curr⌝
+                                             ∗ ⌜es' = es⌝ end),
+                RET (match success with true => SOMEV #() 
+                                      | false => NONEV end)  >>>)%I.
+  
+    Parameter createNode_spec : ∀ (k: nat) (n: Node),
+       ⊢ ({{{ True }}}
+             createNode #k #n
+         {{{ e m es pc, RET #e;
+                node e m es pc
+              ∗ ⌜k ∈ pc⌝
+              ∗ ⌜k ∈ es !!! n⌝ }}})%I.
+  
+    Parameter try_constraint_insert_spec : ∀ (k: nat) (pred curr entry: Node),
+       ⊢ (<<< ∀∀ m es pc, node pred m es pc >>>
+             try_constraint #pred #curr #entry @ ⊤
+         <<< ∃∃ (success: bool) es',
+                node pred m es' pc
+              ∗ (match success with true => ⌜m = false⌝ ∗ ⌜k ∈ es !!! curr⌝
+                                            ∗ ⌜es' = edgset_update es k curr entry⌝ 
+                                  | false => ⌜m = true ∨ k ∉ es !!! curr⌝
+                                             ∗ ⌜es' = es⌝ end),
+                RET (match success with true => SOMEV #() 
+                                      | false => NONEV end)  >>>)%I.   
+    
+    Definition dsG0 : dsG Σ.
+    try done.
+    Admitted.
+    
+End SKIPLIST0.
